Progress on Clight_safety.init_mem_ok.

concurrency/juicy/Clight_safety.v
@@ -19,6 +19,7 @@ Require Import VST.concurrency.common.ClightMachine.
 Require Import VST.concurrency.common.dry_machine_lemmas.
 Require Import VST.concurrency.juicy.semax_simlemmas.
 Require Import VST.concurrency.juicy.semax_to_juicy_machine.
+Require Import VST.concurrency.juicy.mem_wd2.
 Require Import VST.veric.Clight_sim.
 Require Import VST.msl.eq_dec.
 Require Import BinNums.
@@ -638,8 +639,7 @@ Qed.
 Definition mem_ok m := Smallstep.globals_not_fresh (Clight.genv_genv ge) m /\
   (* Mem.mem_wd m isn't sufficient, because there may be values that aren't currently readable
     but will still be used later *)
-  forall b ofs, memval_inject (Mem.flat_inj (Mem.nextblock m))
-    (ZMap.get ofs (Mem.mem_contents m) # b) (ZMap.get ofs (Mem.mem_contents m) # b).
+  mem_wd2 m.
 
 Lemma mem_ok_wd: forall m, mem_ok m -> Mem.mem_wd m.
 Proof.
@@ -659,7 +659,7 @@ Proof.
   destruct H as [? Hwd]; split.
   - unfold Smallstep.globals_not_fresh.
     rewrite restrPermMap_nextblock; auto.
-  - rewrite restrPermMap_nextblock, restrPermMap_mem_contents; auto.
+  - unfold mem_wd2 in *; rewrite restrPermMap_nextblock, restrPermMap_mem_contents; auto.
 Qed.
 
 Lemma mem_ok_step: forall st m st' m' (Hmem: mem_ok m),
@@ -677,44 +677,22 @@ Proof.
       erewrite Mem.nextblock_alloc, restrPermMap_nextblock by eauto.
       etransitivity; eauto.
       apply Ple_succ.
-    + intros.
-      erewrite Mem.nextblock_alloc, restrPermMap_nextblock by eauto.
-      destruct (eq_dec b0 b); [subst; erewrite AllocContentsUndef1 by eauto | erewrite AllocContentsOther1 by eauto].
-      * constructor.
-      * eapply memval_inject_incr, flat_inj_incr, Ple_succ; eauto.
+    + eapply mem_wd2_alloc; eauto.
   - inv Htstep.
     admit.
   - inv Htstep; auto.
-    + destruct Hmem as [? Hwd]; split.
+    + eapply mem_ok_restr in Hmem as [? Hwd]; split.
       * unfold Smallstep.globals_not_fresh.
-        erewrite Mem.nextblock_store, restrPermMap_nextblock; eauto.
-      * intros.
-        erewrite Mem.nextblock_store, restrPermMap_nextblock, Mem.store_mem_contents by eauto.
-        destruct (eq_dec b0 b); [subst; rewrite PMap.gss | rewrite PMap.gso; auto].
-        replace ofs0 with (ofs0 + 0) at 2 by apply Z.add_0_r.
-        replace (Ptrofs.intval ofs) with (Ptrofs.intval ofs + 0) at 3 by apply Z.add_0_r.
-        apply Mem.setN_inj with (access := fun _ => True); intros; rewrite ?Z.add_0_r; auto.
-        apply encode_val_inject; constructor.
-    + destruct Hmem as [? Hwd]; split.
+        erewrite Mem.nextblock_store; eauto.
+      * eapply mem_wd2_store; eauto; simpl; auto.
+    + eapply mem_ok_restr in Hmem as [? Hwd]; split.
       * unfold Smallstep.globals_not_fresh.
-        erewrite Mem.nextblock_store, restrPermMap_nextblock; eauto.
-      * intros.
-        erewrite Mem.nextblock_store, restrPermMap_nextblock, Mem.store_mem_contents by eauto.
-        destruct (eq_dec b0 b); [subst; rewrite PMap.gss | rewrite PMap.gso; auto].
-        replace ofs0 with (ofs0 + 0) at 2 by apply Z.add_0_r.
-        replace (Ptrofs.intval ofs) with (Ptrofs.intval ofs + 0) at 3 by apply Z.add_0_r.
-        apply Mem.setN_inj with (access := fun _ => True); intros; rewrite ?Z.add_0_r; auto.
-        apply encode_val_inject; constructor.
-    + destruct Hmem as [? Hwd]; split.
+        erewrite Mem.nextblock_store; eauto.
+      * eapply mem_wd2_store; eauto; simpl; auto.
+    + eapply mem_ok_restr in Hmem as [? Hwd]; split.
       * unfold Smallstep.globals_not_fresh.
-        erewrite Mem.nextblock_store, restrPermMap_nextblock; eauto.
-      * intros.
-        erewrite Mem.nextblock_store, restrPermMap_nextblock, Mem.store_mem_contents by eauto.
-        destruct (eq_dec b0 b); [subst; rewrite PMap.gss | rewrite PMap.gso; auto].
-        replace ofs0 with (ofs0 + 0) at 2 by apply Z.add_0_r.
-        replace (Ptrofs.intval ofs) with (Ptrofs.intval ofs + 0) at 2 by apply Z.add_0_r.
-        apply Mem.setN_inj with (access := fun _ => True); intros; rewrite ?Z.add_0_r; auto.
-        apply encode_val_inject; constructor.
+        erewrite Mem.nextblock_store; eauto.
+      * eapply mem_wd2_store; eauto; simpl; auto.
 Admitted.
 
 (* spawn handler *)
@@ -1167,7 +1145,20 @@ Qed.
 
 Lemma init_mem_ok: mem_ok init_mem.
 Proof.
-  
+  unfold mem_ok, init_mem, semax_to_juicy_machine.init_mem, init_mem_not_none, CSL_init_mem_not_none,
+    semax_initial.init_m, ge, prog.
+  destruct CPROOF; simpl.
+  destruct (Genv.init_mem CSL_prog) eqn: Hinit; try contradiction; simpl.
+  split.
+  - unfold Smallstep.globals_not_fresh; simpl.
+    erewrite Genv.init_mem_genv_next by eauto.
+    apply Ple_refl.
+  - unfold Genv.init_mem in Hinit.
+    eapply mem_wd2_alloc_globals; eauto.
+    + unfold mem_wd2; simpl; intros.
+      rewrite PMap.gi, ZMap.gi; constructor.
+    + admit. (* Is this designed incorrectly? Why should the genv be valid wrt
+                the memory before allocating globals? *)
 Admitted.
 
 Transparent getThreadC.
